Prove index

src/program_proof/tulip/program/index/index.v
@@ -1,17 +1,26 @@
-From Perennial.program_proof.tulip Require Import prelude.
-From Perennial.program_proof.tulip.program Require Import tuple.
-From Goose.github_com.mit_pdos.tulip Require Import index.
+From Perennial.program_proof.tulip.program Require Import prelude.
+From Perennial.program_proof.tulip.program.tuple Require Import res tuple.
 
 Section program.
   Context `{!heapGS Σ, !tulip_ghostG Σ}.
 
-  Definition is_index (idx : loc) (γ : tulip_names) (α : replica_names) : iProp Σ.
-  Admitted.
+  (*@ type Index struct {                                                     @*)
+  (*@     mu   *sync.Mutex                                                    @*)
+  (*@     tplm map[string]*tuple.Tuple                                        @*)
+  (*@ }                                                                       @*)
+  Definition own_index (idx : loc) γ α : iProp Σ :=
+    ∃ (tplmP : loc) (tplm : gmap dbkey loc),
+      let keys_unalloc := keys_all ∖ (dom tplm) in
+      "HtplmP"  ∷ idx ↦[Index :: "tplm"] #tplmP ∗
+      "Htplm"   ∷ own_map tplmP (DfracOwn 1) tplm ∗
+      "Hphysm"  ∷ ([∗ set] key ∈ keys_unalloc, own_phys_hist_half α key [None]) ∗
+      "#Hreplm" ∷ ([∗ set] key ∈ keys_all, is_repl_hist_lb γ key [None]) ∗
+      "#Htpls"  ∷ ([∗ map] key ↦ tpl ∈ tplm, is_tuple tpl key γ α).
 
-  #[global]
-  Instance is_index_persistent idx γ α :
-    Persistent (is_index idx γ α).
-  Admitted.
+  Definition is_index (idx : loc) (γ : tulip_names) (α : replica_names) : iProp Σ :=
+    ∃ (muP : loc),
+      "#HmuP" ∷ readonly (idx ↦[Index :: "mu"] #muP) ∗
+      "#Hmu"  ∷ is_lock tulipNS #muP (own_index idx γ α).
 
   Theorem wp_Index__GetTuple (idx : loc) (key : string) γ α :
     key ∈ keys_all ->
@@ -20,10 +29,101 @@ Section program.
       Index__GetTuple #idx #(LitString key)
     {{{ (tpl : loc), RET #tpl; is_tuple tpl key γ α }}}.
   Proof.
-    (*@ func (idx *Index) GetTuple(key string) *Tuple {                         @*)
-    (*@     // TODO                                                             @*)
-    (*@     return &Tuple{}                                                     @*)
+    iIntros (Hkey) "#Hidx".
+    iIntros (Φ) "!> _ HΦ".
+    wp_rec.
+
+    (*@ func (idx *Index) GetTuple(key string) *tuple.Tuple {                   @*)
+    (*@     idx.mu.Lock()                                                       @*)
+    (*@     tpl, ok := idx.tplm[key]                                            @*)
+    (*@                                                                         @*)
+    iNamed "Hidx".
+    wp_loadField.
+    wp_apply (wp_Mutex__Lock with "Hmu").
+    iIntros "[Hlocked Hidx]".
+    iNamed "Hidx".
+    wp_loadField.
+    wp_apply (wp_MapGet with "Htplm").
+    iIntros (tplP ok) "[%Hok Htplm]".
+    wp_pures.
+
+    (*@     // Return the tuple if there already exists one.                    @*)
+    (*@     if ok {                                                             @*)
+    (*@         idx.mu.Unlock()                                                 @*)
+    (*@         return tpl                                                      @*)
+    (*@     }                                                                   @*)
+    (*@                                                                         @*)
+    destruct ok; wp_pures.
+    { wp_loadField.
+      wp_apply (wp_Mutex__Unlock with "[-HΦ]").
+      { by iFrame "Hmu Hlocked ∗ #". }
+      wp_pures.
+      iApply "HΦ".
+      apply map_get_true in Hok.
+      by iApply (big_sepM_lookup with "Htpls").
+    }
+    apply map_get_false in Hok as [Hnone _].
+
+    (*@     tplnew := tuple.MkTuple()                                           @*)
+    (*@     idx.tplm[key] = tplnew                                              @*)
+    (*@                                                                         @*)
+    iDestruct (big_sepS_delete _ _ key with "Hphysm") as "[Hphys Hphysm]".
+    { apply not_elem_of_dom in Hnone. set_solver. }
+    iDestruct (big_sepS_elem_of with "Hreplm") as "#Hrepl".
+    { apply Hkey. }
+    wp_apply (wp_MkTuple with "Hrepl Hphys").
+    iIntros (tplnewP) "#Htplnew".
+    wp_loadField.
+    wp_apply (wp_MapInsert with "Htplm"); first done.
+    iIntros "Htplm".
+    iDestruct (big_sepM_insert_2 with "[] Htpls") as "Htpls'".
+    { iFrame "Htplnew". }
+
+    (*@     idx.mu.Unlock()                                                     @*)
+    (*@     return tplnew                                                       @*)
     (*@ }                                                                       @*)
-  Admitted.
+    wp_loadField.
+    wp_apply (wp_Mutex__Unlock with "[-HΦ]").
+    { iFrame "Hmu Hlocked ∗ #".
+      by rewrite dom_insert_L union_comm_L -difference_difference_l_L.
+    }
+    wp_pures.
+    by iApply "HΦ".
+  Qed.
+
+  Theorem wp_MkIndex γ α :
+    ([∗ set] key ∈ keys_all, is_repl_hist_lb γ key [None]) -∗
+    {{{ ([∗ set] key ∈ keys_all, own_phys_hist_half α key [None]) }}}
+      MkIndex #()
+    {{{ (idx : loc), RET #idx; is_index idx γ α }}}.
+  Proof.
+    iIntros "#Hreplm" (Φ) "!> Hphysm HΦ".
+    wp_rec.
+
+    (*@ func MkIndex() *Index {                                                 @*)
+    (*@     idx := new(Index)                                                   @*)
+    (*@     idx.mu = new(sync.Mutex)                                            @*)
+    (*@     idx.tplm = make(map[string]*tuple.Tuple)                            @*)
+    (*@     return idx                                                          @*)
+    (*@ }                                                                       @*)
+    wp_apply wp_allocStruct; first by auto.
+    iIntros (idxP) "Hidx".
+    iDestruct (struct_fields_split with "Hidx") as "Hidx".
+    iNamed "Hidx". simpl.
+    wp_apply wp_new_free_lock.
+    iIntros (muP) "Hfree".
+    wp_storeField.
+    wp_apply wp_NewMap.
+    iIntros (tplmP) "Htplm".
+    wp_storeField.
+    iMod (alloc_lock _ _ _ (own_index idxP γ α) with "Hfree [-HΦ mu]") as "#Hmu".
+    { iFrame "∗ #".
+      rewrite dom_empty_L difference_empty_L big_sepM_empty.
+      by iFrame.
+    }
+    iMod (readonly_alloc_1 with "mu") as "#HmuP".
+    iApply "HΦ".
+    by iFrame "#".
+  Qed.
 
 End program.
